{"nbformat":4,"nbformat_minor":0,"metadata":{"colab":{"provenance":[],"authorship_tag":"ABX9TyOlqpYpLvaECtUMenZ6yJuV"},"kernelspec":{"name":"python3","display_name":"Python 3"},"language_info":{"name":"python"}},"cells":[{"cell_type":"code","execution_count":1,"metadata":{"id":"wIU3g5xvwHmj","executionInfo":{"status":"ok","timestamp":1736254046353,"user_tz":-330,"elapsed":535,"user":{"displayName":"sumantth sumantthkona","userId":"06933787330981542069"}},"outputId":"37647d97-2cac-4e71-8d0e-0661a1b0e7dd","colab":{"base_uri":"https://localhost:8080/"}},"outputs":[{"output_type":"stream","name":"stdout","text":["b1: 2.2572786186088454 b0: 3.4818859195435516\n"]}],"source":["import numpy as np\n","X = np.asarray([20, 5, 10, 13, 12])\n","Y = np.asarray([44, 22, 25, 32, 37])\n","\n","b1 = 0\n","b0 = 0\n","L = 0.001\n","epochs = 1000\n","n = np.size(X)\n","\n","for i in range(epochs):\n","    Y_pred = b1 * X + b0\n","    D_b1 = (-2 / n) * sum(X * (Y - Y_pred))\n","    D_b0 = (-2 / n) * sum((Y - Y_pred))\n","    b1 = b1 - L * D_b1\n","    b0 = b0 - L * D_b0\n","\n","print(\"b1:\", b1, \"b0:\", b0)\n"]}]}